Implement renumbering (wrong)

src/translation/Veriloggen.v
@@ -17,60 +17,258 @@
  *)
 
 From compcert Require Import Maps.
-From compcert Require Errors.
+From compcert Require Import Errors.
 From compcert Require Import AST.
-From vericert Require Import Verilog HTL Vericertlib AssocMap ValueInt.
+From vericert Require Import Vericertlib AssocMap ValueInt Statemonad.
+From vericert Require Import HTL Verilog.
 
-Definition transl_datapath_fun (a : node * HTL.datapath_stmnt) :=
+Record state: Type := mkstate {
+                  st_freshreg : reg;
+                  st_regmap : PTree.t reg;
+                    }.
+
+Module VerilogState <: State.
+  Definition st := state.
+
+  Definition st_prop (st1 st2 : state) := True.
+
+  Lemma st_refl : forall (s : state), st_prop s s.
+  Proof. constructor. Qed.
+
+  Lemma st_trans : forall s1 s2 s3, st_prop s1 s2 -> st_prop s2 s3 -> st_prop s1 s3.
+  Proof. constructor. Qed.
+End VerilogState.
+Export VerilogState.
+
+Module VerilogMonad := Statemonad(VerilogState).
+Export VerilogMonad.
+
+Module VerilogMonadExtra := Monad.MonadExtra(VerilogMonad).
+Import VerilogMonadExtra.
+Export MonadNotation.
+
+Definition renumber_reg (r : reg) : mon reg :=
+  do st <- get;
+  match PTree.get r st.(st_regmap) with
+  | Some reg' => ret reg'
+  | None =>
+    do _ <- set (mkstate (Pos.succ st.(st_freshreg)) st.(st_regmap)) (fun _ => I);
+    ret st.(st_freshreg)
+  end.
+
+Definition transl_datapath_fun (a : Verilog.node * HTL.datapath_stmnt) :=
   let (n, s) := a in
-  (Vlit (posToValue n),
+  (Verilog.Vlit (posToValue n),
    match s with
-   | HTLcall m args dst => Vskip
-   | HTLVstmnt s => s
+   | HTL.HTLcall m args dst => Verilog.Vskip (* inline_call m args *)
+   | HTL.HTLVstmnt s => s
    end).
-
 
 Definition transl_datapath st := map transl_datapath_fun st.
 
-Definition transl_ctrl_fun (a : node * Verilog.stmnt) :=
+Definition transl_ctrl_fun (a : Verilog.node * Verilog.stmnt) :=
   let (n, stmnt) := a
-  in (Vlit (posToValue n), stmnt).
+  in (Verilog.Vlit (posToValue n), stmnt).
 
 Definition transl_ctrl st := map transl_ctrl_fun st.
 
-Definition scl_to_Vdecl_fun (a : reg * (option io * scl_decl)) :=
-  match a with (r, (io, VScalar sz)) => (Vdecl io r sz) end.
+Definition scl_to_Vdecl_fun (a : reg * (option Verilog.io * Verilog.scl_decl)) :=
+  match a with (r, (io, Verilog.VScalar sz)) => (Verilog.Vdecl io r sz) end.
 
 Definition scl_to_Vdecl scldecl := map scl_to_Vdecl_fun scldecl.
 
-Definition arr_to_Vdeclarr_fun (a : reg * (option io * arr_decl)) :=
-  match a with (r, (io, VArray sz l)) => (Vdeclarr io r sz l) end.
+Definition arr_to_Vdeclarr_fun (a : reg * (option Verilog.io * Verilog.arr_decl)) :=
+  match a with (r, (io, Verilog.VArray sz l)) => (Verilog.Vdeclarr io r sz l) end.
 
 Definition arr_to_Vdeclarr arrdecl := map arr_to_Vdeclarr_fun arrdecl.
 
-Definition transl_module (m : HTL.module) : Verilog.module :=
-  let case_el_ctrl := transl_ctrl (PTree.elements m.(mod_controllogic)) in
-  let case_el_data := transl_datapath (PTree.elements m.(mod_datapath)) in
-  let body :=
-      Valways (Vposedge m.(mod_clk)) (Vcond (Vbinop Veq (Vvar m.(mod_reset)) (Vlit (ZToValue 1)))
-                                               (Vnonblock (Vvar m.(mod_st)) (Vlit (posToValue m.(mod_entrypoint))))
-                                               (Vcase (Vvar m.(mod_st)) case_el_ctrl (Some Vskip)))
-      :: Valways (Vposedge m.(mod_clk)) (Vcase (Vvar m.(mod_st)) case_el_data (Some Vskip))
-      :: List.map Vdeclaration (arr_to_Vdeclarr (AssocMap.elements m.(mod_arrdecls))
-                          ++ scl_to_Vdecl (AssocMap.elements m.(mod_scldecls))) in
-  Verilog.mkmodule m.(mod_start)
-                   m.(mod_reset)
-                   m.(mod_clk)
-                   m.(mod_finish)
-                   m.(mod_return)
-                   m.(mod_st)
-                   m.(mod_stk)
-                   m.(mod_stk_len)
-                   m.(mod_params)
-                   body
-                   m.(mod_entrypoint).
+Definition find_module (program : HTL.program) (name : ident) : mon HTL.module :=
+  match option_map snd (find (fun named_module => Pos.eqb (fst named_module) name) program.(prog_defs)) with
+  | Some (Gfun (Internal f)) => ret f
+  | _ => error (Errors.msg "Veriloggen: Could not find definition for called module")
+  end.
 
-Definition transl_fundef := transf_fundef transl_module.
+Fixpoint renumber_edge (edge : Verilog.edge) :=
+  match edge with
+  | Vposedge r =>
+    do r' <- renumber_reg r;
+    ret (Vposedge r')
+  | Vnegedge r =>
+    do r' <- renumber_reg r;
+    ret (Vposedge r')
+  | Valledge => ret Valledge
+  | Voredge e1 e2 =>
+    do e1' <- renumber_edge e1;
+    do e2' <- renumber_edge e2;
+    ret (Voredge e1' e2')
+  end.
 
-Definition transl_program (p: HTL.program) : Verilog.program :=
-  transform_program transl_fundef p.
+Definition renumber_declaration (decl : Verilog.declaration) :=
+  match decl with
+  | Vdecl io reg sz =>
+    do reg' <- renumber_reg reg;
+    ret (Vdecl io reg' sz)
+  | Vdeclarr io reg sz len =>
+    do reg' <- renumber_reg reg;
+    ret (Vdeclarr io reg' sz len)
+  end.
+
+
+Fixpoint renumber_expr (expr : Verilog.expr) :=
+  match expr with
+  | Vlit val => ret (Vlit val)
+  | Vvar reg =>
+    do reg' <- renumber_reg reg;
+    ret (Vvar reg')
+  | Vvari reg e =>
+    do reg' <- renumber_reg reg;
+    do e' <- renumber_expr e;
+    ret (Vvari reg' e')
+  | Vinputvar reg =>
+    do reg' <- renumber_reg reg;
+    ret (Vvar reg')
+  | Vbinop op e1 e2 =>
+    do e1' <- renumber_expr e1;
+    do e2' <- renumber_expr e2;
+    ret (Vbinop op e1' e2')
+  | Vunop op e =>
+    do e' <- renumber_expr e;
+    ret (Vunop op e)
+  | Vternary e1 e2 e3 =>
+    do e1' <- renumber_expr e1;
+    do e2' <- renumber_expr e2;
+    do e3' <- renumber_expr e3;
+    ret (Vternary e1' e2' e3')
+  end.
+
+Fixpoint renumber_stmnt (stmnt : Verilog.stmnt) :=
+  match stmnt with
+  | Vskip => ret Vskip
+  | Vseq s1 s2 =>
+    do s1' <- renumber_stmnt s1;
+    do s2' <- renumber_stmnt s2;
+    ret (Vseq s1' s2')
+  | Vcond e s1 s2 =>
+    do e' <- renumber_expr e;
+    do s1' <- renumber_stmnt s1;
+    do s2' <- renumber_stmnt s2;
+    ret (Vcond e' s1' s2')
+  | Vcase e cs def =>
+    do e' <- renumber_expr e;
+    do cs' <- sequence (map
+                            (fun (c : (Verilog.expr * Verilog.stmnt)) =>
+                           let (c_expr, c_stmnt) := c in
+                           do expr' <- renumber_expr c_expr;
+                           do stmnt' <- renumber_stmnt c_stmnt;
+                           ret (expr', stmnt')) cs);
+    do def' <- match def with
+              | None => ret None
+              | Some d => do def' <- renumber_stmnt d; ret (Some def')
+              end;
+    ret (Vcase e' cs' def')
+  | Vblock e1 e2 =>
+    do e1' <- renumber_expr e1;
+    do e2' <- renumber_expr e2;
+    ret (Vblock e1' e2')
+  | Vnonblock e1 e2 =>
+    do e1' <- renumber_expr e1;
+    do e2' <- renumber_expr e2;
+    ret (Vnonblock e1' e2')
+  end.
+
+Definition renumber_module_item (item : Verilog.module_item) :=
+  match item with
+  | Vdeclaration decl =>
+    do decl' <- renumber_declaration decl;
+    ret (Vdeclaration decl')
+  | Valways edge stmnt =>
+    do edge' <- renumber_edge edge;
+    do stmnt' <- renumber_stmnt stmnt;
+    ret (Valways edge' stmnt')
+  | Valways_ff edge stmnt =>
+    do edge' <- renumber_edge edge;
+    do stmnt' <- renumber_stmnt stmnt;
+    ret (Valways edge' stmnt')
+  | Valways_comb edge stmnt =>
+    do edge' <- renumber_edge edge;
+    do stmnt' <- renumber_stmnt stmnt;
+    ret (Valways edge' stmnt')
+  end.
+
+
+Definition renumber_module (m : Verilog.module) : mon Verilog.module :=
+  do mod_start' <- renumber_reg (Verilog.mod_start m);
+  do mod_reset' <- renumber_reg (Verilog.mod_reset m);
+  do mod_clk' <- renumber_reg (Verilog.mod_clk m);
+  do mod_finish' <- renumber_reg (Verilog.mod_finish m);
+  do mod_return' <- renumber_reg (Verilog.mod_return m);
+  do mod_st' <- renumber_reg (Verilog.mod_st m);
+  do mod_stk' <- renumber_reg (Verilog.mod_stk m);
+  do mod_args' <- traverselist renumber_reg (Verilog.mod_args m);
+  let mod_body' := (Verilog.mod_body m) in
+
+  ret (Verilog.mkmodule
+     mod_start'
+     mod_reset'
+     mod_clk'
+     mod_finish'
+     mod_return'
+     mod_st'
+     mod_stk'
+     (Verilog.mod_stk_len m)
+     mod_args'
+     mod_body'
+     (Verilog.mod_entrypoint m)).
+
+
+Definition called_functions : (list (Verilog.node * HTL.datapath_stmnt)) -> list ident :=
+  flat_map (fun (a : (positive * HTL.datapath_stmnt)) =>
+          let (n, stmt) := a in
+          match stmt with
+          | HTL.HTLcall fn _ _ => fn::nil
+          | _ => nil
+          end).
+
+(* FIXME Remove the fuel parameter (recursion limit)*)
+Fixpoint transf_module (fuel : nat) (program : HTL.program) (m : HTL.module) : mon Verilog.module :=
+  match fuel with
+  | O => error (Errors.msg "Veriloggen: transl_module ran out of fuel")
+  | S fuel' =>
+    let case_el_ctrl := transl_ctrl (PTree.elements (HTL.mod_controllogic m)) in
+    let case_el_data := transl_datapath (PTree.elements (HTL.mod_datapath m)) in
+
+    (* Inlining *)
+    let inline_names := called_functions (PTree.elements (HTL.mod_datapath m)) in
+    do inline_modules <- traverselist (find_module program) inline_names;
+    do translated_modules <- traverselist (transf_module fuel' program) inline_modules;
+    do renumbered_modules <- traverselist renumber_module translated_modules;
+
+    let body :=
+        Valways (Vposedge (HTL.mod_clk m)) (Vcond (Vbinop Veq (Vvar (HTL.mod_reset m)) (Vlit (ZToValue 1)))
+                                                  (Vnonblock (Vvar (HTL.mod_st m)) (Vlit (posToValue (HTL.mod_entrypoint m))))
+                                                  (Vcase (Vvar (HTL.mod_st m)) case_el_ctrl (Some Vskip)))
+                :: Valways (Vposedge (HTL.mod_clk m)) (Vcase (Vvar (HTL.mod_st m)) case_el_data (Some Vskip))
+                :: List.map Vdeclaration (arr_to_Vdeclarr (AssocMap.elements (HTL.mod_arrdecls m))
+                                                         ++ scl_to_Vdecl (AssocMap.elements (HTL.mod_scldecls m)))
+                ++ List.flat_map (fun m => (Verilog.mod_body m)) renumbered_modules in
+
+    ret (Verilog.mkmodule
+       (HTL.mod_start m)
+       (HTL.mod_reset m)
+       (HTL.mod_clk m)
+       (HTL.mod_finish m)
+       (HTL.mod_return m)
+       (HTL.mod_st m)
+       (HTL.mod_stk m)
+       (HTL.mod_stk_len m)
+       (HTL.mod_params m)
+       body
+       (HTL.mod_entrypoint m)
+        )
+  end.
+
+Definition transl_module (prog : HTL.program) (m : HTL.module) :=
+  run_mon (mkstate xH (PTree.empty reg)) (transf_module 10 prog m).
+
+Definition transl_fundef (prog : HTL.program) := transf_partial_fundef (transl_module prog).
+Definition transl_program (prog : HTL.program) := transform_partial_program (transl_fundef prog) prog.
