src/translation/Veriloggenproof.v
@@ -17,14 +17,18 @@
  *)
 
 From compcert Require Import Smallstep Linking Integers Globalenvs.
+From compcert Require Errors.
 From vericert Require HTL.
 From vericert Require Import Vericertlib Veriloggen Verilog ValueInt AssocMap.
 Require Import Lia.
 
+
 Local Open Scope assocmap.
 
 Definition match_prog (prog : HTL.program) (tprog : Verilog.program) :=
-  match_program (fun cu f tf => tf = transl_fundef f) eq prog tprog.
+  match_program (fun cu f tf => Errors.OK tf = transl_fundef prog f) eq prog tprog.
+
+(*
 
 Lemma transf_program_match:
   forall prog, match_prog prog (transl_program prog).
@@ -404,3 +408,4 @@ Section CORRECTNESS.
   Qed.
 
 End CORRECTNESS.
+*)
